src/ecDecl.mli
@@ -95,6 +95,7 @@ type axiom = {
 
 (* -------------------------------------------------------------------- *)
 type typeclass = {
+  tc_prt : EcPath.path option;
   tc_ops : (EcIdent.t * EcTypes.ty) list;
   tc_axs : (EcSymbols.symbol * form) list;
 }
